sepcomp/linking_lemmas.v
@@ -32,14 +32,6 @@ case: st=> fn_tbl; case; case=> //= a l pf.
 by case: a pf=> ? c pf /=; do 2 f_equal=> //=; apply: proof_irr.
 Qed.
 
-(*Lemma peek_upd' (st : Linker.linker N cores) : 
-  let: c := peekCore st in
-  updCore st (peekCore (Core.upd c c)) = st.
-Proof.
-case: st=> fn_tbl; case; case=> //= a l pf.
-by case: a pf=> ? c pf /=; do 2 f_equal=> //=; apply: proof_irr.
-Qed.*)
-
 Lemma upd_peek (st : Linker.linker N cores) c : peekCore (updCore st c) = c.
 Proof. by []. Qed.
 
@@ -58,6 +50,7 @@ Proof.
 move=> STEP; move: (@effstep_corestep _ _ _ _ _ _ _ _ _ STEP)=> STEP'; split.
 by left; exists c1'; split.
 by move=> ?; exists c1'; split.
+by move=> H b ofs; case: H; rewrite/Sem.corestep0; exists c1'; split.
 Qed.
 
 Lemma stepN_STEPN {U st1 m1 c1' m1' n} :
@@ -69,14 +62,15 @@ Lemma stepN_STEPN {U st1 m1 c1' m1' n} :
   n U st1 m1 (updCore st1 (Core.upd c1 c1')) m1'.
 Proof.
 move: st1 c1' m1 U; elim: n.
-case=> ?; case; case=> //; case=> ? a l ? /= ? ? ?; case=> <- <-.
-by do 3 f_equal; apply: proof_irr.
-move=> n IH st1 c1' m1 U /= => [][]c1'' []m1'' []B C.
-exists (updCore st1 (Core.upd (peekCore st1) c1'')), m1''; split.
+case=> ?; case; case=> // a l pf x ? ?; case; case=> /= <- <- <-; split=> //.
+do 3 f_equal. move=> // _ _; case=> <- <-; f_equal=> //.
+by move: pf x; case: a=> //. 
+by apply: proof_irr.
+move=> n IH st1 c1' m1 U /= => [][]c1'' []m1'' []U1 []U2 []B []C D.
+exists (updCore st1 (Core.upd (peekCore st1) c1'')), m1'',U1,U2; split.
 by apply: (step_STEP B).
-set U' := fun b ofs => U b ofs || StructuredInjections.freshloc m1 m1'' b.
-move: (IH (updCore st1 (Core.upd (peekCore st1) c1'')) c1' m1'' U'). 
-by rewrite upd_upd; apply.
+move: (IH (updCore st1 (Core.upd (peekCore st1) c1'')) c1' m1'' U2).
+by rewrite upd_upd=> H; split=> //; move: H; apply; apply: C.
 Qed.
 
 Lemma stepPLUS_STEPPLUS {U st1 m1 c1' m1'} :
